{-# OPTIONS --without-K #-}

module Container where

open import lib.Base
open import lib.types.Sigma

infix 5 _â—_

record Container : Type1 where
  constructor _â—_
  field
    Sh : Type0
    Ps : Sh â†’ Type0

-- Functorial actions
module _ where
  -- Action on objects
  âŸ¦_âŸ§â‚€ : Container â†’ Type0 â†’ Type0
  âŸ¦_âŸ§â‚€ (Sh â— Ps) X = Î£ Sh (Î» s â†’ Ps s â†’ X)

  -- Action on morphisms
  âŸ¦_âŸ§â‚ : {X Y : Type0} â†’ (F : Container) â†’ (X â†’ Y) â†’ âŸ¦ F âŸ§â‚€ X â†’ âŸ¦ F âŸ§â‚€ Y
  âŸ¦_âŸ§â‚ (Sh â— Ps) f (s , t) = (s , f âˆ˜ t)

record ContHom (A B : Container) : Type0 where
  constructor mk-cont-hom
  open Container A
  open Container B renaming (Sh to Th ; Ps to Qs)
  field
    sh : Sh â†’ Th
    ps : (s : Sh) â†’ Qs (sh s) â†’ Ps s

apply : {F G : Container} (Î± : ContHom F G) (X : Type0) â†’ âŸ¦ F âŸ§â‚€ X â†’ âŸ¦ G âŸ§â‚€ X
apply (mk-cont-hom sh ps) X (s , t) = sh s , t âˆ˜ (ps s)

_â€¼_ : {F G : Container} (Î± : ContHom F G) {X : Type0} â†’ âŸ¦ F âŸ§â‚€ X â†’ âŸ¦ G âŸ§â‚€ X
_â€¼_ Î± {X} = apply Î± X

module _ (F : Container) where
  open Container F

  â–¡ : {A : Type0} (B : A â†’ Type0) â†’ âŸ¦ F âŸ§â‚€ A â†’ Type0
  â–¡ B (s , t) = (p : Ps s) â†’ B (t p)

  Ï† : {A : Type0} (B : A â†’ Type0) â†’ âŸ¦ F âŸ§â‚€ (Î£ A B) â†’ Î£ (âŸ¦ F âŸ§â‚€ A) (â–¡ B)
  Ï† B (s , t) = (âŸ¦ F âŸ§â‚ fst (s , t)) , (Î» p â†’ snd (t p))

  Ï†â»Â¹ : {A : Type0} (B : A â†’ Type0) â†’ Î£ (âŸ¦ F âŸ§â‚€ A) (â–¡ B) â†’ âŸ¦ F âŸ§â‚€ (Î£ A B)
  Ï†â»Â¹ B ((s , t) , p) = s , (Î» x â†’ (t x) , (p x))
  
  bar : {A : Type0} {B : A â†’ Type0}
    â†’ ((x : A) â†’ B x) â†’ (x : âŸ¦ F âŸ§â‚€ A) â†’ â–¡ B x
  bar ğ“¼ (s , t) = Î» p â†’ ğ“¼ (t p)
  
  open import lib.Funext using (Î»=)

  postulate
    Î»=-idp :
      {A : Type0}
      {P : A â†’ Type0}
      (f : Î  A P) â†’ Î»= (Î» x â†’ idp {a = f x}) == idp

  lift-func-eq :
    {A B : Type0} (f g : A â†’ B)
    (x : âŸ¦ F âŸ§â‚€ A) (y : â–¡ (Î» x' â†’ f x' == g x') x)
    â†’ âŸ¦ F âŸ§â‚ f x == âŸ¦ F âŸ§â‚ g x
  lift-func-eq f g (s , t) h = ap (Î» p â†’ s , p) (Î»= h)

  lift-func-eq-idp :
    {A B : Type0}
    (f : A â†’ B)
    (x : âŸ¦ F âŸ§â‚€ A) 
    â†’ lift-func-eq f f x (Î» _ â†’ idp) == idp
  lift-func-eq-idp f (s , t) =
    ap (Î» h â†’ ap (Î» p â†’ s , p) h) (Î»=-idp _)
