{-# OPTIONS --without-K #-}

open import Container

-- Equality of algebra morphisms
module 1-hits.Alg0.Eq.Core (F : Container) where

open import lib.Basics
open import 1-hits.Alg0.Core F

private
  module Prim
    (ğ“§ ğ“¨ : Algâ‚€-obj)
    where

    open Algâ‚€-obj ğ“§
    open Algâ‚€-obj ğ“¨ renaming (X to Y ; Î¸ to Ï)
    open Algâ‚€-hom

    algâ‚€-hom= :
      (ğ“¯ ğ“° : Algâ‚€-hom ğ“§ ğ“¨)
      (p : f ğ“¯ == f ğ“°)
      (pâ‚€ : (fâ‚€ ğ“¯) == (fâ‚€ ğ“°) [ is-algâ‚€-hom ğ“§ ğ“¨ â†“ p ])
      â†’ ğ“¯ == ğ“°
    algâ‚€-hom= (algâ‚€-hom f fâ‚€) (algâ‚€-hom .f gâ‚€) idp = ap (algâ‚€-hom f)
  
module _
  {ğ“§ ğ“¨ : Algâ‚€-obj}
  where

  record =Algâ‚€-hom (ğ“¯ ğ“° : Algâ‚€-hom ğ“§ ğ“¨) : Type0 where
    constructor =algâ‚€-hom

    open Algâ‚€-obj ğ“§
    open Algâ‚€-obj ğ“¨ renaming (X to Y ; Î¸ to Ï)
    open Algâ‚€-hom ğ“¯
    open Algâ‚€-hom ğ“° renaming (f to g ; fâ‚€ to gâ‚€)

    field
      p  : f == g
      pâ‚€ : fâ‚€ == gâ‚€ [ is-algâ‚€-hom ğ“§ ğ“¨ â†“ p ]

  algâ‚€-hom= : (ğ“¯ ğ“° : Algâ‚€-hom ğ“§ ğ“¨) â†’ =Algâ‚€-hom ğ“¯ ğ“° â†’ ğ“¯ == ğ“°
  algâ‚€-hom= ğ“¯ ğ“° (=algâ‚€-hom p pâ‚€) = Prim.algâ‚€-hom= ğ“§ ğ“¨ ğ“¯ ğ“° p pâ‚€

-- (ğ“¯ == ğ“°) â‰ƒ =Algâ‚€-hom ğ“¯ ğ“°
open Algâ‚€-hom
open Algâ‚€-obj

f= :
  {ğ“§ ğ“¨ : Algâ‚€-obj}
  {ğ“¯ ğ“° : Algâ‚€-hom ğ“§ ğ“¨}
  â†’ ğ“¯ == ğ“° â†’ (f ğ“¯) == (f ğ“°)
f= ğ“¹ = ap f ğ“¹
  
fâ‚€= :
  {ğ“§ ğ“¨ : Algâ‚€-obj}
  {ğ“¯ ğ“° : Algâ‚€-hom ğ“§ ğ“¨}
  (ğ“¹ : ğ“¯ == ğ“°)
  â†’ fâ‚€ ğ“¯ == fâ‚€ ğ“° [ is-algâ‚€-hom ğ“§ ğ“¨ â†“ f= ğ“¹ ]
fâ‚€= idp = idp

f=-Î² :
  {ğ“§ ğ“¨ : Algâ‚€-obj}
  {ğ“¯ ğ“° : Algâ‚€-hom ğ“§ ğ“¨}
  (p : f ğ“¯ == f ğ“°)
  (pâ‚€ : fâ‚€ ğ“¯ == fâ‚€ ğ“° [ is-algâ‚€-hom ğ“§ ğ“¨ â†“ p ])
  â†’ f= (algâ‚€-hom= ğ“¯ ğ“° (=algâ‚€-hom p pâ‚€)) == p
f=-Î² idp idp = idp

fâ‚€=-Î² :
  {ğ“§ ğ“¨ : Algâ‚€-obj}
  {ğ“¯ ğ“° : Algâ‚€-hom ğ“§ ğ“¨}
  (p : f ğ“¯ == f ğ“°)
  (pâ‚€ : fâ‚€ ğ“¯ == fâ‚€ ğ“° [ is-algâ‚€-hom ğ“§ ğ“¨ â†“ p ])
  â†’ fâ‚€= (algâ‚€-hom= ğ“¯ ğ“° (=algâ‚€-hom p pâ‚€)) == pâ‚€ [ (Î» p' â†’ fâ‚€ ğ“¯ == fâ‚€ ğ“° [ is-algâ‚€-hom ğ“§ ğ“¨ â†“ p' ]) â†“ f=-Î² p pâ‚€ ]
fâ‚€=-Î² idp idp = idp

algâ‚€-hom=-Î· :
  {ğ“§ ğ“¨ : Algâ‚€-obj}
  {ğ“¯ ğ“° : Algâ‚€-hom ğ“§ ğ“¨}
  (ğ“¹ : ğ“¯ == ğ“°)
  â†’ ğ“¹ == algâ‚€-hom= ğ“¯ ğ“° (=algâ‚€-hom (f= ğ“¹) (fâ‚€= ğ“¹))
algâ‚€-hom=-Î· idp = idp
